\section{Introducing OPP}
    \subsection{Class}

    \subsection{Object}

\section{Inheritence}

\section{Examples}

In \emref{eq.2}{Eq } if 
\begin{equation}
    y(t)=\phi^T(t)\theta(t) + e(t)
\end{equation}
such that, $e(t)$ is a white noise with zero mean and variance $\sigma^2$, then
\begin{align*}
    \hat{\theta}(i) = \theta + \left(\sum_{j=1}^{i}\varphi(j)\varphi^T(j)\right)^{-1}\left(\sum_{j=1}^{i}\varphi(j)e(j)\right).
\end{align*}
therefore, 
\begin{equation}
    E\{\hat{\theta}\}=\theta .
\end{equation}
On the other hand we know that
\begin{align}
    \mathrm{var}(\hat{\theta}) = E\{\hat{\theta}^2\} - E^2\{\hat{\theta}\}.
\end{align}
\begin{proof}
We expand the given equation on both side:
\begin{align}
    E\{(\hat{\theta}-\theta)^2\} &= E\{\hat{\theta}^2 + \theta^2 - 2\theta\hat{\theta}\}\\
    &= E\{\hat{\theta}^2\} + E\{\theta^2\} - 2E\{\theta\hat{\theta}\} \nonumber\\
    &= \theta^2 + E\{\hat{\theta}^2\} - 2\theta E\{\hat{\theta}\}.\nonumber\\
    &\nonumber\\
    bias^2 + var &= (\theta - E\{\hat{\theta}\})^2 + E\{\hat{\theta}^2\} - E^2\{\hat{\theta}\}\\
    &= \theta^2 + E\{\hat{\theta}^2\} - 2\theta E\{\hat{\theta}\}.\nonumber
\end{align}
The both side of equation are equal, so the proof is complete.
\end{proof}